working SK translation

theories/CombinatoryLogic/CL.v
@@ -1,6 +1,518 @@
 From Undecidability Require L.L.
-Require Import List.
+Require Import List Lia.
 Import L (var, app, lam).
+
+(* direct one full reduction *)
+
+Inductive eterm : Type :=
+  | eK : eterm
+  | eS : eterm
+  | evar (n : nat) : eterm
+  | eapp (s : eterm) (t : eterm) : eterm.
+
+(* stream cons *)
+Definition scons {X: Type} (x : X) (xi : nat -> X) :=
+  fun n => match n with | 0 => x | S n => xi n end.
+
+Fixpoint eren (xi : nat -> nat) (t : eterm) : eterm  :=
+  match t with
+  | evar x => evar (xi x)
+  | eapp s t => eapp (eren xi s) (eren xi t)
+  | _ => t
+  end.
+
+  (*
+Fixpoint ren (xi : nat -> nat) (t : L.term) : L.term  :=
+  match t with
+  | var x => var (xi x)
+  | app s t => app (ren xi s) (ren xi t)
+  | lam t => lam (ren (scons 0 xi) t)
+  end.
+*)
+(* variable capturing substitution : bad idea *)
+Fixpoint esubst' (s : eterm) (k : nat) (u : eterm) :=
+  match s with
+    | evar n => if Nat.eqb n k then u else evar n
+    | eapp s t => eapp (esubst' s k u) (esubst' t k u)
+    | _ => s
+  end.
+
+Definition closed' s := forall n t, esubst' s n t = s.
+
+Inductive evalue : eterm -> Prop :=
+  | evalue_K0 : evalue eK
+  | evalue_K1 t : evalue (eapp eK t)
+  | evalue_S0 : evalue eS
+  | evalue_S1 t : evalue (eapp eS t)
+  | evalue_S2 s t : evalue (eapp (eapp eS s) t).
+
+(* capturing definitions *)
+
+Inductive estep : eterm -> eterm -> Prop :=
+  | estepK  s t       : evalue t -> estep (eapp (eapp eK s) t) s
+  | estepS  s t u     : evalue u -> estep (eapp (eapp (eapp eS s) t) u) (eapp (eapp s u) (eapp t u))
+  | estepAppR s t  t' : estep t t' -> estep (eapp s t) (eapp s t')
+  | estepAppL s s' t  : estep s s' -> estep (eapp s t) (eapp s' t).
+  
+Fixpoint contains_evar n (t : eterm) : bool :=
+  match t with
+  | evar m => if Nat.eqb n m then true else false
+  | eapp s t => contains_evar n s || contains_evar n t
+  | _ => false
+  end.
+(*
+Fixpoint contains_var n (t : L.term) : bool :=
+  match t with
+  | var m => if Nat.eqb n m then true else false
+  | app s t => contains_var n s || contains_var n t
+  | lam t => contains_var (S n) t
+  end.
+*)
+(* working abstraction *)
+Fixpoint abstraction (s : eterm) : eterm :=
+  if contains_evar 0 s then
+    match s with
+    | evar 0 => eapp (eapp eS eK) eK
+    | eapp s t => eapp (eapp eS (abstraction s)) (abstraction t)
+    | _ => eapp eK s
+    end else eapp eK (eren Nat.pred s).
+
+Fixpoint translate (s : L.term) : eterm :=
+  match s with
+  | var n => evar n
+  | app s t => eapp (translate s) (translate t)
+  | lam t => abstraction (translate t)
+  end.
+
+  Require Import Relations PeanoNat.
+  #[local] Arguments clos_trans {A}.
+  From Undecidability Require L.Util.L_facts.
+Require Import ssreflect ssrbool ssrfun.
+Unset Implicit Arguments.
+
+Lemma evalue_abstraction t : evalue (abstraction t).
+Proof.
+  elim: t => /=.
+  - by auto using evalue.
+  - by auto using evalue.
+  - case; by auto using evalue.
+  - move=> s ? t ?.
+    move: (contains_evar 0 s) (contains_evar 0 t) => [] [] /=; by auto using evalue.
+Qed.
+
+Lemma closed'_eappE s t : closed' (eapp s t) -> closed' s /\ closed' t.
+Proof. move=> H. split => n u; by have [] := H n u. Qed.
+
+Lemma closed'_eappI s t : closed' s -> closed' t -> closed' (eapp s t).
+Proof. move=> Hs Ht n u /=. by rewrite (Hs n u) (Ht n u). Qed.
+
+Lemma many_estepAppL s t u : clos_trans estep s t -> clos_trans estep (eapp s u) (eapp t u).
+Proof.
+  elim.
+  - move=> > /estepAppL ?. by apply: t_step.
+  - move=> > ????. by apply: t_trans; eassumption.
+Qed.
+
+Lemma many_estepAppR s t u : clos_trans estep s t -> clos_trans estep (eapp u s) (eapp u t).
+Proof.
+  elim.
+  - move=> > /estepAppR ?. by apply: t_step.
+  - move=> > ????. by apply: t_trans; eassumption.
+Qed.
+
+Lemma closed'_evarE n : closed' (evar n) -> False.
+Proof. move=> /(_ n eK) /=. by rewrite Nat.eqb_refl. Qed.
+
+Lemma closed'_erenE xi t : closed' (eren xi t) -> closed' t.
+Proof.
+  elim: t; [done|done| |].
+  - by move=> > /closed'_evarE.
+  - move=> ? IH1 ? IH2.
+    move=> /closed'_eappE [/IH1 + /IH2].
+    by apply: closed'_eappI.
+Qed.
+
+Lemma closed'_eren xi {t} : closed' t -> eren xi t = t.
+Proof.
+  elim: t; [done|done| |].
+  - by move=> > /closed'_evarE.
+  - move=> /= ? IH1 ? IH2.
+    by move=> /closed'_eappE [/IH1 -> /IH2 ->].
+Qed.
+
+Lemma estep_abstraction s t :
+  evalue t -> closed' (abstraction s) -> clos_trans estep (eapp (abstraction s) t) (esubst' s 0 t).
+Proof.
+  move=> Ht. elim: s.
+  - move=> ?. apply: t_step. by apply: estepK.
+  - move=> ?. apply: t_step. by apply: estepK.
+  - move=> [|n] /= H.
+    + apply: t_trans. { apply: t_step. by apply: estepS. }
+      apply: t_step. apply: estepK. by apply: evalue_K1.
+    + exfalso. move: H => /closed'_eappE [_].
+      move=> /(_ n eK) /=. by rewrite Nat.eqb_refl.
+  - move=> s1 IH1 s2 IH2.
+    case Hs1s2: (contains_evar 0 (eapp s1 s2)).
+    + move: Hs1s2 => /= ->.
+      move=> /closed'_eappE [/closed'_eappE] [_].
+      move=> /IH1 {}IH1 /IH2 {}IH2.
+      apply: t_trans. { apply: t_step. by apply: estepS. }
+      apply: t_trans. { apply: many_estepAppL. by eassumption. }
+      by apply: many_estepAppR.
+    + move: (Hs1s2) => /= ->.
+      move=> /closed'_eappE [_] /closed'_eappE [] /closed'_erenE Hs1 /closed'_erenE Hs2.
+      move: Hs1 Hs2 (Hs1) (Hs2) => -> -> /closed'_eren -> /closed'_eren ->.
+      apply: t_step. by apply: estepK.
+Qed.
+
+Lemma closed'_not_contains_evar t n : closed' t -> contains_evar n t = false.
+Proof.
+  elim: t; [done|done| |].
+  - by move=> > /closed'_evarE.
+  - by move=> s IH1 t IH2 /closed'_eappE /= [/IH1 -> /IH2 ->].
+Qed.
+
+Lemma esubst'_eren_pred s n t : closed' t -> contains_evar 0 s = false ->
+  esubst' (eren Nat.pred s) n t = eren Nat.pred (esubst' s (S n) t).
+Proof.
+  move=> Ht. elim: s; [done|done| |].
+  - move=> [|m]; first done.
+    move=> _ /=. case: (Nat.eqb m n); last done.
+    by rewrite (closed'_eren Nat.pred Ht).
+  - move=> s1 IH1 s2 IH2 /=.
+    by move=> /norP [/negPf /IH1 -> /negPf /IH2 ->].
+Qed.
+
+Lemma contains_evar_0_esubst' s n t : closed' t ->
+  contains_evar 0 (esubst' s (S n) t) = contains_evar 0 s.
+Proof.
+  move=> Ht. elim: s; [done|done| |].
+  - move=> [|m] /=; first done.
+    case: (Nat.eqb m n); last done.
+    by apply: closed'_not_contains_evar.
+  - by move=> /= s1 -> s2 ->.
+Qed.
+
+Lemma esubst'_abstraction s n t :
+  closed' t ->
+  esubst' (abstraction s) n t = abstraction (esubst' s (S n) t).
+Proof.
+  move=> Ht. elim: s n; [done|done| |].
+  - move=> [|m] n /=; first done.
+    case E: (Nat.eqb m n); last done.
+    case: t Ht => > /= ; [done|done| |].
+    + by move=> /closed'_evarE.
+    + move=> /closed'_eappE [H1 H2].
+      move: (H1) (H2) => /closed'_eren -> /closed'_eren ->.
+      by move: H1 H2 => /closed'_not_contains_evar -> /closed'_not_contains_evar ->.
+  - move=> s1 IH1 s2 IH2 n.
+    case Hs1s2: (contains_evar 0 (eapp s1 s2)).
+    + rewrite /= !contains_evar_0_esubst' //.
+      move: Hs1s2 => /= ->. by rewrite /= IH1 IH2.
+    + rewrite /= !contains_evar_0_esubst' //.
+      move: (Hs1s2) => /= ->.
+      move: Hs1s2 => /= /norP [/negPf ? /negPf ?].
+      by rewrite !esubst'_eren_pred.
+Qed.
+
+Lemma not_contains_evar_closed' t : (forall n, contains_evar n t = false) -> closed' t.
+Proof.
+  elim: t; [done|done| |].
+  - move=> m /(_ m) /=. by rewrite Nat.eqb_refl.
+  - move=> /= s IH1 t IH2 H. apply: closed'_eappI.
+    + apply: IH1 => n. by have /norP [/negPf ->] := H n.
+    + apply: IH2 => n. by have /norP [_ /negPf ->] := H n.
+Qed.
+
+Lemma contains_evar_pred n t : contains_evar 0 t = false ->
+  contains_evar n (eren Nat.pred t) = contains_evar (S n) t.
+Proof.
+  elim: t; [done|done|by case|].
+  by move=> s IH1 t IH2 /= /norP [/negPf /IH1 -> /negPf /IH2 ->].
+Qed.
+
+Lemma contains_evar_abstraction n s : contains_evar n (abstraction s) = contains_evar (S n) s.
+Proof.
+  elim: s; [done|done|by case|].
+  move=> s IH1 t IH2.
+  case H: (contains_evar 0 (eapp s t)).
+  - move: H => /= -> /=. by rewrite IH1 IH2.
+  - move: (H) => /= -> /=.
+    by move: H => /= /norP [/negPf /contains_evar_pred -> /negPf /contains_evar_pred ->].
+Qed.
+
+Lemma closed'_translate s : L_facts.closed s -> closed' (translate s).
+Proof.
+  move=> /L_facts.closed_dcl Hs.
+  apply: not_contains_evar_closed' => n.
+  have : 0 <= n by lia.
+  move: (0) Hs n => ?. elim.
+  - move=> m x ? n /= ?.
+    by have /Nat.eqb_neq -> : n <> x by lia.
+  - move=> > ? IH1 ? IH2 ?? /=.
+    rewrite IH1; [done|]. by rewrite IH2.
+  - move=> > ? IH n ? /=.
+    rewrite contains_evar_abstraction. apply: IH. lia.
+Qed.
+
+Lemma esubst'_translate s n t : L_facts.closed t ->
+  esubst' (translate s) n (translate t) = translate (L.subst s n t).
+Proof.
+  move=> Ht. elim: s n => /=.
+  - move=> m n. by case: (Nat.eqb m n).
+  - move=> s1 IH1 s2 IH2 n. by rewrite IH1 IH2.
+  - move=> s IH n. rewrite esubst'_abstraction. { by apply: closed'_translate. }
+    by rewrite IH.
+Qed.
+
+(* transforms a goal (A -> B) -> C into goals A and B -> C *)
+Lemma unnest : forall (A B C : Type), A -> (B -> C) -> (A -> B) -> C.
+Proof. auto. Qed.
+
+(* actually plus instead of star *)
+(* this can be shown *)
+Lemma main s t : L_facts.step s t -> L_facts.closed s ->
+  clos_trans estep (translate s) (translate t).
+Proof.
+  elim.
+  - move=> {}s {}t /= /L_facts.closed_app [Hs Ht].
+    have /(estep_abstraction (translate s)) := evalue_abstraction (translate t).
+    apply: unnest. { by apply: (closed'_translate (lam s)). }
+    congr clos_trans.
+    by apply: (esubst'_translate _ _ (lam t)).
+  - move=> > ? IH /L_facts.closed_app [_ /IH] /=.
+    by apply: many_estepAppR.
+  - move=> > ? IH /L_facts.closed_app [/IH + _] /=.
+    by apply: many_estepAppL.
+Qed.
+
+Print Assumptions main.
+
+Inductive eval : term -> term -> Prop :=
+| eval_abs s : eval (lam s) (lam s)
+| eval_app s u t t' v :
+    eval s (lam u) -> eval t t' -> eval (subst u 0 t') v -> eval (app s t) v.
+    
+Inductive term : Type :=
+  | term_K : eterm
+  | term_S : eterm
+  | term_app (s : eterm) (t : eterm) : eterm.
+
+(*
+OBSOLETE
+
+
+
+(* exponential translation, doesnt fully work *)
+Fixpoint abstraction (s : eterm) : eterm :=
+  match s with
+  | evar 0 => eapp (eapp eS eK) eK
+  | evar (S n) => eapp eK (evar n)
+  | eapp s t => eapp (eapp eS (abstraction s)) (abstraction t)
+  | _ => eapp eK s
+  end.
+
+Fixpoint translate (s : L.term) : eterm :=
+  match s with
+  | var n => evar n
+  | app s t => eapp (translate s) (translate t)
+  | lam t => abstraction (translate t)
+  end.
+
+  Require Import Relations PeanoNat.
+  #[local] Arguments clos_trans {A}.
+  From Undecidability Require L.Util.L_facts.
+Require Import ssreflect ssrbool ssrfun.
+Unset Implicit Arguments.
+
+Lemma evalue_abstraction t : evalue (abstraction t).
+Proof.
+  elim: t => /=.
+  - by auto using evalue.
+  - by auto using evalue.
+  - case; by auto using evalue.
+  - by auto using evalue.
+Qed.
+
+Lemma closed'_eapp s t : closed' (eapp s t) -> closed' s /\ closed' t.
+Proof. Admitted.
+
+Lemma many_estepAppL s t u : clos_trans estep s t -> clos_trans estep (eapp s u) (eapp t u).
+Proof.
+  elim.
+  - move=> > /estepAppL ?. by apply: t_step.
+  - move=> > ????. by apply: t_trans; eassumption.
+Qed.
+
+Lemma many_estepAppR s t u : clos_trans estep s t -> clos_trans estep (eapp u s) (eapp u t).
+Proof.
+  elim.
+  - move=> > /estepAppR ?. by apply: t_step.
+  - move=> > ????. by apply: t_trans; eassumption.
+Qed.
+
+Lemma estep_abstraction s t :
+  evalue t -> closed' (abstraction s) -> clos_trans estep (eapp (abstraction s) t) (esubst' s 0 t).
+Proof.
+  move=> Ht. elim: s => /=.
+  - move=> ?. apply: t_step. by apply: estepK.
+  - move=> ?. apply: t_step. by apply: estepK.
+  - move=> [|n] /= H.
+    + apply: t_trans. { apply: t_step. by apply: estepS. }
+      apply: t_step. apply: estepK. by apply: evalue_K1.
+    + exfalso. move: H => /closed'_eapp [_].
+      move=> /(_ n eK) /=. by rewrite Nat.eqb_refl.
+  - move=> s1 IH1 s2 IH2 /closed'_eapp [/closed'_eapp [_]].
+    move=> /IH1 {}IH1 /IH2 {}IH2.
+    apply: t_trans. { apply: t_step. by apply: estepS. }
+    apply: t_trans. { apply: many_estepAppL. by eassumption. }
+    by apply: many_estepAppR.
+Qed.
+
+Lemma aaa s n t :
+closed' t ->
+esubst' (abstraction s) n t =
+abstraction (esubst' s (S n) t).
+Proof.
+  move=> Ht. elim: s n => /=.
+  - done.
+  - done.
+  - move=> [|m] n /=; first done.
+    case E: (Nat.eqb m n); last done.
+    case: t Ht.
+    + done.
+    + done.
+    + admit. (* doable *)
+    + cbn.
+    (* works only if t is closed !!!!!!!!! *)
+    admit.
+  - move=> s1 IH1 s2 IH2 n. by rewrite IH1 IH2.
+Admitted.
+
+Lemma esubst'_translate s n t :
+  L_facts.closed t ->
+  esubst' (translate s) n (translate t) =
+  translate (L.subst s n t).
+Proof.
+  move=> Ht. elim: s n => /=.
+  - move=> m n. by case: (Nat.eqb m n).
+  - move=> s1 IH1 s2 IH2 n. by rewrite IH1 IH2.
+  - move=> s IH n. by rewrite aaa IH.
+Qed.
+
+
+(* transforms a goal (A -> B) -> C into goals A and B -> C *)
+Lemma unnest : forall (A B C : Type), A -> (B -> C) -> (A -> B) -> C.
+Proof. auto. Qed.
+
+
+
+(* actually plus instead of star *)
+(* this can be shown *)
+Lemma main s t : L_facts.step s t -> L_facts.closed s ->
+  clos_trans estep (translate s) (translate t).
+Proof.
+  elim.
+  - move=> {}s {}t /= ?.
+    have /(estep_abstraction (translate s)) := evalue_abstraction (translate t).
+    apply: unnest. { admit. }
+    congr clos_trans.
+    apply: (esubst'_translate _ _ (lam t)).
+  - move=> > ? IH /L_facts.closed_app [_ /IH] /=.
+    by apply: many_estepAppR.
+  - move=> > ? IH /L_facts.closed_app [/IH + _] /=.
+    by apply: many_estepAppL.
+Admitted.
+      
+
+(* full SK translation *)
+Inductive translate : L.term -> eterm -> Prop :=
+  | translate_var n : translate (var n) (evar n)
+  | translate_app s t s' t' : translate s s' -> translate t t' -> translate (app s t) (eapp s' t')
+  | translate_lam_I : translate (lam (var 0)) (eapp (eapp eS eK) eK)
+  | translate_lam_K s s' s'' : s = ren S s' -> translate s' s'' -> translate (lam s) (eapp eK s'')
+  (* this is wrong! S (\s') (\t') *)
+  | translate_lam_S s s' s'' : contains_var 0 s = true -> translate s (eapp s' s'') -> translate (lam s) (eapp (eapp eS s') s'').
+
+  (* domain of translate *)
+Inductive translate_domain : L.term -> Prop :=
+  | translate_domain_var n : translate_domain (var n)
+  | translate_domain_app s t : translate_domain s -> translate_domain t -> translate_domain (app s t)
+  | translate_domain_lam_I : translate_domain (lam (var 0))
+  | translate_domain_lam_K s s' : s = ren S s' -> translate_domain s' -> translate_domain (lam s)
+  | translate_domain_lam_S s : contains_var 0 s = true -> translate_domain s -> translate_domain (lam s).
+
+Definition translate_domainE {s} : translate_domain s -> 
+  match s with
+  | app s' t' => translate_domain s' /\ translate_domain t'
+  | _ => True
+  end :=
+    fun H => match H with
+    | translate_domain_app s t Hs Ht => conj Hs Ht
+    | _ => I
+    end.
+
+
+Fixpoint translate' s (Ds : translate_domain s) {struct Ds} : { t | translate s t }.
+Proof.
+  case: s Ds.
+  - move=> n *. exists (evar n). by apply: translate_var.
+  - move=> s t H. have [Hs Ht] := translate_domainE H.
+    have [s' Hs'] := translate' s Hs.
+    have [t' Ht'] := translate' t Ht.
+    exists (app )
+
+Lemma translate_domain_total s : translate_domain s.
+Proof.
+  elim: s.
+  - by apply: translate_domain_var.
+  - move=> *. by apply: translate_domain_app.
+  - move=> s. case Es: (contains_var 0 s) => [|].
+    { by apply: translate_domain_lam_S. }
+    move=> ?. apply: translate_domain_lam_K.
+    admit. (* doable with some ren *)
+Admitted.
+
+
+  move=> [|n].
+
+  
+  
+
+  
+  (* actually plus instead of star *)
+  (* this can be shown *)
+  Lemma main s t s' t' : estep s t -> closed s ->
+    translate s s' -> translate t t' ->
+    clos_trans estep s' t'.
+  Proof.
+    elim.
+    - move=> {}s {}t /=.
+      move=> /SK_evalue /estepK H ?. exists 1. by apply /t_step /H.
+    - move=> {}s {}t u /=.
+      move=> /SK_evalue /estepS H ?. exists 1. by apply /t_step /H.
+    - move=> {}s {}t Ht /=.
+      case Es: (contains_evar 0 s) => [|]; first last.
+      { move=> ?. exists 0 => /=.
+        apply: t_step.
+        move: Ht => /SK_evalue /estepK.
+        admit. (* actually doable because s' is closed and renamings do nothing
+        apply: ARS.starR.*) }
+      case: s Es.
+      + done.
+      + done.
+      + move=> [|n] ??; last done.
+        exists 1 => /=.
+        apply: t_trans; [apply: t_step|]. { apply: estepS. by apply: SK_evalue. }
+        apply: t_step. apply: estepK. by apply: evalue_K1.
+      + move=> {}s u ?? /=. exists 1 => /=.
+        apply: t_trans; [apply: t_step|]. { apply: estepS. by apply: SK_evalue. }
+        apply: t_trans; [apply: t_step|]. { apply: estepAppR. apply: estepApp. by apply: SK_evalue. }
+        apply: t_trans; [apply: t_step|]. { apply: estepAppL. apply: estepApp. by apply: SK_evalue. }
+        (* BREAKS DOWN! *)
+        
+
+(* old multistep reduction *)
 
 (*
 (* S/K_term t1 .. tn = S/K t1 .. tn *)
@@ -92,6 +604,172 @@ Proof.
 Admitted.
 *)
 
+(* based on first elam term: does not work because of S s [t] u <> s [u] (t u) 
+based on both terms does not work because (\x.F G) H does wrongly translate H
+*)
+
+(* full SK translation *)
+Inductive translate : L.term -> eterm -> Prop :=
+  | translate_eK : translate (lam (var 0)) eK.
+  | translate_eS : translate eS eS
+  | translate_evar n : translate (evar n) (evar n)
+  | translate_eapp s t s' t' : translate s s' -> translate t t' -> translate (eapp s t) (eapp s' t')
+  | translate_elam_I : translate (elam (evar 0)) (eapp (eapp eS eK) eK)
+  | translate_elam_K s s' s'' : s = eren S s' -> translate s' s'' -> translate (elam s) (eapp eK s'')
+  | translate_elam_S s s' s'' : contains_evar 0 s = true -> translate s (eapp s' s'') -> translate (elam s) (eapp (eapp eS s') s'').
+
+(* domain of translate *)
+Inductive translate_domain : eterm -> Prop :=
+  | translate_domain_eK : translate_domain eK
+  | translate_domain_eS : translate_domain eS
+  | translate_domain_evar n : translate_domain (evar n)
+  | translate_domain_eapp s t : translate_domain s -> translate_domain t -> translate_domain (eapp s t)
+  | translate_domain_elam_I : translate_domain (elam (evar 0))
+  | translate_domain_elam_K s s' : s = eren S s' -> translate_domain s' -> translate_domain (elam s)
+  | translate_domain_elam_S s : contains_evar 0 s = true -> translate_domain s -> translate_domain (elam s).
+
+
+
+From Undecidability Require L.Util.L_facts.
+Require Import ssreflect ssrbool ssrfun.
+Require Import Relations.
+#[local] Arguments clos_trans {A}.
+
+(* actually plus instead of star *)
+(* this can be shown *)
+Lemma main s t s' t' : estep s t -> closed s ->
+  translate s s' -> translate t t' ->
+  clos_trans estep s' t'.
+Proof.
+  elim.
+  - move=> {}s {}t /=.
+    move=> /SK_evalue /estepK H ?. exists 1. by apply /t_step /H.
+  - move=> {}s {}t u /=.
+    move=> /SK_evalue /estepS H ?. exists 1. by apply /t_step /H.
+  - move=> {}s {}t Ht /=.
+    case Es: (contains_evar 0 s) => [|]; first last.
+    { move=> ?. exists 0 => /=.
+      apply: t_step.
+      move: Ht => /SK_evalue /estepK.
+      admit. (* actually doable because s' is closed and renamings do nothing
+      apply: ARS.starR.*) }
+    case: s Es.
+    + done.
+    + done.
+    + move=> [|n] ??; last done.
+      exists 1 => /=.
+      apply: t_trans; [apply: t_step|]. { apply: estepS. by apply: SK_evalue. }
+      apply: t_step. apply: estepK. by apply: evalue_K1.
+    + move=> {}s u ?? /=. exists 1 => /=.
+      apply: t_trans; [apply: t_step|]. { apply: estepS. by apply: SK_evalue. }
+      apply: t_trans; [apply: t_step|]. { apply: estepAppR. apply: estepApp. by apply: SK_evalue. }
+      apply: t_trans; [apply: t_step|]. { apply: estepAppL. apply: estepApp. by apply: SK_evalue. }
+      (* BREAKS DOWN! *)
+      
+      
+      apply: ARS.starC.
+        apply: estepS. done.
+        apply: ARS.starC.
+        apply: estepAppR.
+        apply: estepApp. done.
+        apply: ARS.starC.
+        apply: estepAppL.
+        apply: estepApp. done.
+        apply: ARS.starR.
+    + move=> s Es ?.
+      exists 1.
+      apply: ARS.starC.
+      apply: estepApp. done.
+      rewrite esubst'_SK_step. admit. (* easy *)
+      apply: ARS.starR.
+  - move=> {}s {}t u Htu IH /closed_eappE [? /IH] /=.
+    move=> [n Hn].
+    move E: (contains_elam s) => [].
+    + exists 1 => /=.
+      rewrite E.
+      apply: ARS.starC.
+      apply: estepAppR. eassumption.
+      apply: ARS.starR.
+    + exists n. admit. (* easy *)
+  - move=> {}s {}t u Hst IH /closed_eappE [/IH [n Hn] ?].
+    admit. (* difficult, doable *)
+Admitted.
+
+
+
+(*
+Lemma esubst_not_contains_evar {s n t} : 
+  contains_evar n s = false ->
+  esubst s n t = s.
+Proof.
+  elim: s n.
+Admitted.
+*)
+Lemma closed_eappE s t : closed (eapp s t) -> closed s /\ closed t.
+Proof.
+Admitted.
+
+Lemma closed_contains_evar {n t} : closed t -> contains_evar n t = false.
+Proof.
+Admitted.
+
+Lemma SK_step_elam_false t : contains_evar 0 t = false -> SK_step (elam t) = eapp eK (eren Nat.pred t).
+Proof. by move=> /= ->. Qed.
+
+Lemma SK_step_elam_true t : contains_evar 0 t = true -> SK_step (elam t) = 
+  match t with
+  | eapp t1 t2 => eapp (eapp eS (elam t1)) (elam t2)
+  | elam _ => elam (SK_step t)
+  | _ => eapp (eapp eS eK) eK
+  end.
+Proof. by move=> /= ->. Qed.
+
+Lemma esubst'elam s t n : esubst' (elam s) n t = elam (esubst' s (S n) t).
+Proof. done. Qed.
+
+Lemma esubst'eapp s1 s2 t n : esubst' (eapp s1 s2) n t = eapp (esubst' s1 n t) (esubst' s2 n t).
+Proof. done. Qed.
+
+Lemma esubst'_SK_step n s t : closed t -> esubst' (SK_step (elam s)) n t = SK_step (esubst' (elam s) n t).
+Proof.
+  elim: s n.
+  - done.
+  - done.
+  - move=> [|m] n Ht /=; first done.
+    case Emn: (Nat.eqb m n) => [|] /=.
+    + rewrite (closed_contains_evar Ht).
+     admit. (* easy *)
+    + done.
+  - move=> s1 IH1 s2 IH2 n Ht.
+    case E: (contains_evar 0 (eapp s1 s2)) => [|].
+    * move: (E) => /SK_step_elam_true ->.
+     rewrite esubst'elam.
+     rewrite SK_step_elam_true. admit. (* doable *)
+      rewrite  !esubst'eapp.
+      done.
+    * move: (E) => /SK_step_elam_false ->.
+    rewrite esubst'elam.
+    rewrite SK_step_elam_false. admit. (* doable *)
+    simpl.
+    admit. (* doable *)
+  - move=> s IH n Ht.
+    case Es: (contains_evar 0 (elam s)) => [|].
+    + move: (Es) => /SK_step_elam_true ->.
+      rewrite !esubst'elam IH. done.
+      rewrite SK_step_elam_true. admit. (* doable *)
+      done.
+    + move: (Es) => /SK_step_elam_false ->.
+      rewrite !esubst'elam.
+      rewrite SK_step_elam_false. admit. (* doable *)
+      cbn. congr eapp.
+      congr elam.
+      admit. (* doable *)
+Admitted.
+
+
+
+(* based on first elam term: does not work because of S s [t] u <> s [u] (t u) *)
+
 Fixpoint SK_step (t : eterm) : eterm :=
   match t with
     | eapp s t => if contains_elam s then eapp (SK_step s) t else eapp s (SK_step t)
@@ -105,9 +783,8 @@ Fixpoint SK_step (t : eterm) : eterm :=
     | _ => t
   end.
 
-From Undecidability Require L.Util.L_facts.
-Require Import ssreflect ssrbool ssrfun.
-From Undecidability Require L.Prelim.ARS.
+
+
 
 Lemma SK_step_not_contains_elam {t} : contains_elam t = false ->
   SK_step t = t.
@@ -186,19 +863,29 @@ Proof.
       admit. (* doable *)
 Admitted.
 
+#[local] Arguments clos_trans {A}.
 
 (* actually plus instead of star *)
 (* this can be shown *)
 Lemma main s t : estep s t -> closed s ->
-  exists n, ARS.star estep (SK_step s) (Nat.iter n SK_step t).
+  exists n, clos_trans estep (SK_step s) (Nat.iter n SK_step t).
 Proof.
   elim.
   - move=> {}s {}t /=. move E: (contains_elam s) => [].
-    + move=> /estepK H ?. exists 1. by apply: ARS.starC; [|apply: ARS.starR].
-    + move=> /SK_evalue /estepK H ?. exists 1 => /=.
-      move: E => /SK_step_not_contains_elam ->.
-      by apply: ARS.starC; [|apply: ARS.starR].
-  - admit.
+    + move=> /estepK ??. exists 1. by apply: t_step.
+    + move=> /SK_evalue /estepK ??. exists 1.
+      move: E => /SK_step_not_contains_elam /= ->.
+      by apply: t_step.
+  - move=> {}s {}t u /=. move Es: (contains_elam s) => [] /=.
+    + move=> /estepS ??. exists 1. apply: t_step.
+      by rewrite /= Es /=.
+    + move Et: (contains_elam t) => [].
+      * move=> /estepS ??. exists 1. apply: t_step.
+        rewrite /= Es /=.
+      
+      move=> /SK_evalue /estepK ??. exists 1.
+      move: E => /SK_step_not_contains_elam /= ->.
+      by apply: t_step.
   - move=> {}s {}t Ht /=.
     case Es: (contains_evar 0 s) => [|]; first last.
     { move=> ?. exists 0 => /=.
@@ -651,3 +1338,4 @@ Proof.
 
 Print translation.
 *)
+
